\(p \ra q \land r \vdash (p \ra q) \land (p \ra r)\)
\begin{logicproof}{2}
    p \ra q \land r & premise \label{1prm1}\\
        \begin{subproof}
        p & assumption \label{1p1}\\
        q \land r & \re{\ra} \ref{1p1}, \ref{1prm1}\\
        q & \re[1]{\land} \label{1q}
        \end{subproof}
    p \ra q & \ri{\ra} \ref{1p1}-\ref{1q} \label{1pgq}\\
        \begin{subproof}
        p & assumption \label{1p2}\\
        q \land r & \re{\ra} \ref{1p2}, \ref{1prm1}\\
        r & \re[2]{\land} \label{1r}
        \end{subproof}
    p \ra r & \ri{\ra} \ref{1p2}-\ref{1r} \label{1pgr}\\
    (p \ra q) \land (p \ra r) & \ri{\land} \ref{1pgq}, \ref{1pgr}
\end{logicproof}
~\\ %\vspace{-2mm}
