\begin{tabbing}
boxproof:\\
We wish to prove (p\(\ra\)q)\(\lor\)(q\(\ra\)r).\\
By applying the law of the excluded middle, we get q\(\lor\)\(\neg\)q [1].\\
Ass\=ume \+ q [2].\\ 
	Ass\=ume \+ p [3].\\
		By copying 2, we get q here too [4].\\
	\< \- Discharge assumption [3].\\
	By applying the implication-introduction rule to [3]-[4], we get p\(\ra\)q [5].\\
	By applying the first or-introduction rule to [5], we get (p\(\ra\)q)\(\lor\)(q\(\ra\)r) [6].\\
\< \- Discharge assumption [2].\\
Ass\=ume \+ \(\neg\)q [7].\\
	Ass\=ume \+ q [8].\\
		By applying the negation-elimination rule to [8] and [7], we get \(\bot\) [9].\\
		By applying elimination of absurdity to [9], we get r [10].\\
	\< \- Discharge assumption [8].\\
	By applying the implication-introduction rule to [8]-[10], we get q\(\ra\)r [11].\\
	By applying the second or-introduction rule to [11], we get (p\(\ra\)q)\(\lor\)(q\(\ra\)r) [12].\\
\< \- Discharge assumption [7].\\
By applying the or-elimination rule to [1], [2]-[6], and [7]-[12], we conclude (p\(\ra\)q)\(\lor\)(q\(\ra\)r).
\end{tabbing}
